Progress on loop_to_wordProofs

pancake/proofs/loop_to_wordProofScript.sml
@@ -2,11 +2,12 @@
   Correctness proof for loop_to_word
 *)
 
-open preamble loopLangTheory loopSemTheory loopPropsTheory wordSemTheory wordPropsTheory
+open preamble
+     loopSemTheory loopPropsTheory
+     wordLangTheory wordSemTheory wordPropsTheory
+     pan_commonTheory pan_commonPropsTheory
 
-val _ = new_theory"loop_to_wordProof";
-
-val _ = set_grammar_ancestry ["loopSem","loopProps","wordSem"];
+val _ = new_theory "loop_to_wordProof";
 
 Definition assigned_vars_def:
   (assigned_vars (Seq p1 p2) l = assigned_vars p1 (assigned_vars p2 l)) ∧
@@ -38,29 +39,6 @@ Definition assigned_vars_def:
   (assigned_vars (FFI name n1 n2 n3 n4 live) l = l)
 End
 
-Theorem assigned_vars_acc:
-  ∀p l.
-    domain (assigned_vars p l) = domain (assigned_vars p LN) ∪ domain l
-Proof
-  qsuff_tac ‘∀p (l:num_set) l.
-    domain (assigned_vars p l) = domain (assigned_vars p LN) UNION domain l’
-  >- metis_tac [] >>
-  ho_match_mp_tac assigned_vars_ind >> rw [] >> fs [] >>
-  ntac 4 (once_asm_rewrite_tac [assigned_vars_def]) >>
-  simp_tac (srw_ss()) [domain_def,AC UNION_COMM UNION_ASSOC,domain_union,
-       domain_insert,LET_THM] >>
-  every_case_tac >>
-  simp_tac (srw_ss()) [domain_def,AC UNION_COMM UNION_ASSOC,domain_union,
-       domain_insert,LET_THM] >>
-  once_rewrite_tac [INSERT_SING_UNION] >>
-  simp_tac (srw_ss()) [domain_def,AC UNION_COMM UNION_ASSOC,domain_union,
-       domain_insert,LET_THM] >>
-  rpt (pop_assum (fn th => mp_tac (SIMP_RULE std_ss [] th))) >>
-  rewrite_tac [AND_IMP_INTRO] >>
-  disch_then (fn th => ntac 6 (once_rewrite_tac [th])) >>
-  simp_tac (srw_ss()) [domain_def,AC UNION_COMM UNION_ASSOC,domain_union,
-       domain_insert,LET_THM] >> fs [EXTENSION] >> metis_tac []
-QED
 
 Definition find_var_def:
   find_var ctxt v =
@@ -84,7 +62,7 @@ Termination
   rw [] >>
   rename [‘MEM x xs’] >>
   Induct_on ‘xs’ >> fs [] >>
-  fs [exp_size_def] >>
+  fs [loopLangTheory.exp_size_def] >>
   rw [] >> fs []
 End
 
@@ -97,7 +75,7 @@ Definition fromNumSet_def:
   fromNumSet t = MAP FST (toAList t)
 End
 
-(* Why inserting zero? *)
+(* TOASK: Why inserting zero? *)
 Definition mk_new_cutset_def:
   mk_new_cutset ctxt (l:num_set) =
     insert 0 () (toNumSet (MAP (find_var ctxt) (fromNumSet l)))
@@ -112,9 +90,11 @@ Definition comp_def:
   (comp ctxt (SetGlobal a e) l =
      (Set (Temp a) (comp_exp ctxt e), l)) /\
   (comp ctxt (LoadByte a v) l =
-     (Inst (Mem Load8 v ((Addr a 0w))), l)) /\
+     (Inst (Mem Load8 (find_var ctxt v)
+            (Addr (find_var ctxt a) 0w)), l)) /\
   (comp ctxt (StoreByte a v) l =
-     (Inst (Mem Store8 v ((Addr a 0w))), l)) /\
+     (Inst (Mem Store8 (find_var ctxt v)
+            (Addr (find_var ctxt a) 0w)), l)) /\
   (comp ctxt (Seq p q) l =
     let (wp,l) = comp ctxt p l in
      let (wq,l) = comp ctxt q l in
@@ -149,11 +129,10 @@ Definition comp_def:
                 (Seq (Call (SOME (v,live,p2,l)) dest args
                    (SOME (find_var ctxt n,p1,l1))) Tick, new_l)) /\
    (comp ctxt (FFI f ptr1 len1 ptr2 len2 live) l =
-     (FFI f (find_var ctxt len1) (find_var ctxt ptr2)
-      (find_var ctxt len2) (find_var ctxt len2) live,l))
+     (FFI f (find_var ctxt ptr1) (find_var ctxt len1)
+      (find_var ctxt ptr2) (find_var ctxt len2) live,l))
 End
 
-(* what is make context? from here *)
 Definition make_ctxt_def:
   make_ctxt n [] l = l ∧
   make_ctxt n (x::xs) l = make_ctxt (n+2:num) xs (insert x n l)
@@ -198,35 +177,14 @@ Definition state_rel_def:
     code_rel s.code t.code
 End
 
-Theorem find_var_neq_0:
-  var_name ∈ domain ctxt ∧ locals_rel ctxt l1 l2 ⇒
-  find_var ctxt var_name ≠ 0
-Proof
-  fs [locals_rel_def,find_var_def] \\ rw []
-  \\ Cases_on ‘lookup var_name ctxt’ \\ fs []
-  \\ fs [domain_lookup] \\ res_tac \\ metis_tac []
-QED
-
-Theorem locals_rel_insert:
-  locals_rel ctxt l1 l2 ∧ v IN domain ctxt ⇒
-  locals_rel ctxt (insert v w l1) (insert (find_var ctxt v) w l2)
-Proof
-  fs [locals_rel_def,lookup_insert] \\ rw []
-  \\ fs [CaseEq"bool"] \\ rveq \\ fs []
-  \\ fs [domain_lookup,find_var_def]
-  \\ res_tac \\ fs []
-  \\ disj2_tac \\ CCONTR_TAC \\ fs [] \\ rveq \\ fs []
-  \\ fs [INJ_DEF,domain_lookup]
-  \\ first_x_assum (qspecl_then [‘v’,‘n’] mp_tac)
-  \\ fs [] \\ fs [find_var_def]
-QED
+(* TOASK: l is only being used in comp? *)
 
 val goal =
   ``λ(prog, s). ∀res s1 t ctxt retv l.
       evaluate (prog,s) = (res,s1) ∧ res ≠ SOME Error ∧
       state_rel s t ∧ locals_rel ctxt s.locals t.locals ∧
       lookup 0 t.locals = SOME retv ∧ no_Loops prog ∧
-      ~ (isWord retv) ∧
+      ~(isWord retv) ∧
       domain (assigned_vars prog LN) ⊆ domain ctxt ⇒
       ∃t1 res1.
          evaluate (FST (comp ctxt prog l),t) = (res1,t1) ∧
@@ -259,31 +217,158 @@ in
   fun the_ind_thm () = ind_thm
 end
 
+Theorem locals_rel_intro:
+  locals_rel ctxt l1 l2 ==>
+    INJ (find_var ctxt) (domain ctxt) UNIV ∧
+    (∀n m. lookup n ctxt = SOME m ==> m ≠ 0) ∧
+    ∀n v. lookup n l1 = SOME v ⇒
+          ∃m. lookup n ctxt = SOME m ∧ lookup m l2 = SOME v
+Proof
+  rw [locals_rel_def]
+QED
+
+Theorem globals_rel_intro:
+  globals_rel g1 g2 ==>
+    ∀n v. FLOOKUP g1 n = SOME v ⇒ FLOOKUP g2 (Temp n) = SOME v
+Proof
+  rw [globals_rel_def]
+QED
+
+Theorem code_rel_intro:
+  code_rel s_code t_code ==>
+    ∀name params body.
+      lookup name s_code = SOME (params,body) ⇒
+      lookup name t_code = SOME (LENGTH params+1, compile name params body) ∧
+      no_Loops body ∧ ALL_DISTINCT params
+Proof
+  rw [code_rel_def] >> metis_tac []
+QED
+
+Theorem state_rel_intro:
+  state_rel s t ==>
+    t.memory = s.memory ∧
+    t.mdomain = s.mdomain ∧
+    t.clock = s.clock ∧
+    t.be = s.be ∧
+    t.ffi = s.ffi ∧
+    globals_rel s.globals t.store ∧
+    code_rel s.code t.code
+Proof
+  rw [state_rel_def]
+QED
+
+Theorem find_var_neq_0:
+  v ∈ domain ctxt ∧ locals_rel ctxt lcl lcl' ⇒
+  find_var ctxt v ≠ 0
+Proof
+  fs [locals_rel_def, find_var_def] >> rw [] >>
+  Cases_on ‘lookup var_name ctxt’ >> fs [] >>
+  fs [domain_lookup] >> res_tac >> metis_tac []
+QED
+
+Theorem locals_rel_insert:
+  locals_rel ctxt lcl lcl' ∧ v IN domain ctxt ⇒
+  locals_rel ctxt (insert v w lcl)
+     (insert (find_var ctxt v) w lcl')
+Proof
+  fs [locals_rel_def,lookup_insert] >> rw [] >>
+  fs [CaseEq"bool"] >> rveq >> fs [] >>
+  fs [domain_lookup,find_var_def] >>
+  res_tac >> fs [] >>
+  disj2_tac >> CCONTR_TAC >> fs [] >> rveq >> fs [] >>
+  fs [INJ_DEF,domain_lookup] >>
+  first_x_assum (qspecl_then [‘v’,‘n’] mp_tac) >>
+  fs [] >> fs [find_var_def]
+QED
+
+Theorem locals_rel_get_var:
+  locals_rel ctxt l t.locals ∧ lookup n l = SOME w ⇒
+  wordSem$get_var (find_var ctxt n) t = SOME w
+Proof
+  fs [locals_rel_def] >> rw[] >> res_tac >>
+  fs [find_var_def, get_var_def]
+QED
+
+
+Theorem assigned_vars_acc:
+  ∀p l.
+    domain (assigned_vars p l) = domain (assigned_vars p LN) ∪ domain l
+Proof
+  qsuff_tac ‘∀p (l:num_set) l.
+    domain (assigned_vars p l) = domain (assigned_vars p LN) UNION domain l’
+  >- metis_tac [] >>
+  ho_match_mp_tac assigned_vars_ind >> rw [] >> fs [] >>
+  ntac 4 (once_asm_rewrite_tac [assigned_vars_def]) >>
+  simp_tac (srw_ss()) [domain_def,AC UNION_COMM UNION_ASSOC,domain_union,
+       domain_insert,LET_THM] >>
+  every_case_tac >>
+  simp_tac (srw_ss()) [domain_def,AC UNION_COMM UNION_ASSOC,domain_union,
+       domain_insert,LET_THM] >>
+  once_rewrite_tac [INSERT_SING_UNION] >>
+  simp_tac (srw_ss()) [domain_def,AC UNION_COMM UNION_ASSOC,domain_union,
+       domain_insert,LET_THM] >>
+  rpt (pop_assum (fn th => mp_tac (SIMP_RULE std_ss [] th))) >>
+  rewrite_tac [AND_IMP_INTRO] >>
+  disch_then (fn th => ntac 6 (once_rewrite_tac [th])) >>
+  simp_tac (srw_ss()) [domain_def,AC UNION_COMM UNION_ASSOC,domain_union,
+       domain_insert,LET_THM] >> fs [EXTENSION] >> metis_tac []
+QED
+
+Theorem comp_exp_preserves_eval:
+  !s e v t ctxt.
+   eval s e = SOME v ∧
+   state_rel s t /\ locals_rel ctxt s.locals t.locals ==>
+    word_exp t (comp_exp ctxt e) = SOME v
+Proof
+  ho_match_mp_tac eval_ind >>
+  rw [] >>
+  fs [eval_def, comp_exp_def, word_exp_def]
+  >- (
+   fs [find_var_def, locals_rel_def] >>
+   TOP_CASE_TAC >> fs [] >>
+   first_x_assum drule >>
+   strip_tac >> fs [] >> rveq >> fs [])
+  >- fs [state_rel_def, globals_rel_def]
+  >- (
+   cases_on ‘eval s e’ >> fs [] >>
+   cases_on ‘x’ >> fs [] >>
+   first_x_assum drule_all >> fs [] >>
+   strip_tac >>
+   fs [state_rel_def, mem_load_def,
+       loopSemTheory.mem_load_def])
+  >- (
+   fs [CaseEq "option"] >>
+   qsuff_tac
+   ‘the_words (MAP (λa. word_exp t a)
+               (MAP (λa. comp_exp ctxt a) wexps)) = SOME ws’
+   >- fs [] >>
+   ntac 2 (pop_assum mp_tac) >>
+   ntac 2 (pop_assum kall_tac) >>
+   rpt (pop_assum mp_tac) >>
+   qid_spec_tac ‘ws’ >>
+   qid_spec_tac ‘wexps’ >>
+   Induct >> rw [] >>
+   last_assum mp_tac >>
+   impl_tac >- metis_tac [] >>
+   fs [the_words_def, CaseEq"option", CaseEq"word_loc"] >>
+   rveq >> fs []) >>
+  fs [CaseEq"option", CaseEq"word_loc"] >> rveq >> fs []
+QED
+
+
 Theorem compile_Skip:
   ^(get_goal "comp _ loopLang$Skip") ∧
   ^(get_goal "comp _ loopLang$Fail") ∧
   ^(get_goal "comp _ loopLang$Tick")
 Proof
-  rpt strip_tac
-  THEN1 (
-   fs [loopSemTheory.evaluate_def,comp_def,wordSemTheory.evaluate_def]
-   \\ rveq
-   \\ fs [])
-  THEN1
-   fs [loopSemTheory.evaluate_def,comp_def,wordSemTheory.evaluate_def]
-  \\ fs [loopSemTheory.evaluate_def,comp_def,wordSemTheory.evaluate_def]
-  \\ Cases_on ‘s.clock = 0’
-  \\ fs []
-  \\ rveq
-  THEN1 (
-   IF_CASES_TAC
-   \\ fs [flush_state_def,state_rel_def]
-   \\ rveq
-   \\ fs []
-   )
-  \\ IF_CASES_TAC
-  \\ fs [assigned_vars_def,state_rel_def,
-         wordSemTheory.dec_clock_def,loopSemTheory.dec_clock_def]
+  rpt strip_tac >>
+  fs [loopSemTheory.evaluate_def, comp_def,
+      evaluate_def] >>
+  rveq >> fs [] >>
+  TOP_CASE_TAC >>
+  fs [flush_state_def, state_rel_def,
+      loopSemTheory.dec_clock_def, dec_clock_def] >> rveq >>
+  fs []
 QED
 
 Theorem compile_Loop:
@@ -291,266 +376,241 @@ Theorem compile_Loop:
   ^(get_goal "comp _ loopLang$Break") ∧
   ^(get_goal "comp _ (loopLang$Loop _ _ _)")
 Proof
-  rpt strip_tac
-  \\ fs [no_Loops_def,every_prog_def]
-  \\ fs [no_Loop_def,every_prog_def]
+  rpt strip_tac >>
+  fs [no_Loops_def, every_prog_def] >>
+  fs [no_Loop_def, every_prog_def]
 QED
 
 Theorem compile_Mark:
   ^(get_goal "comp _ (Mark _)")
 Proof
-  rpt strip_tac
-  \\ fs [loopSemTheory.evaluate_def,comp_def,wordSemTheory.evaluate_def,
-         no_Loops_def,assigned_vars_def,no_Loop_def,every_prog_def]
+  rpt strip_tac >>
+  fs [loopSemTheory.evaluate_def, comp_def,
+      evaluate_def, no_Loops_def,
+      assigned_vars_def, no_Loop_def, every_prog_def]
 QED
 
 Theorem compile_Return:
   ^(get_goal "loopLang$Return")
 Proof
-  rpt strip_tac
-  \\ fs [loopSemTheory.evaluate_def,comp_def,wordSemTheory.evaluate_def]
-  \\ Cases_on ‘lookup n s.locals’
-  \\ fs []
-  \\ rveq
-  \\ TOP_CASE_TAC \\ fs [find_var_def,locals_rel_def,get_var_def]
-  \\ res_tac
-  \\ rveq
-  \\ TOP_CASE_TAC \\ fs [isWord_def]
-  \\ fs [flush_state_def,state_rel_def,loopSemTheory.call_env_def]
-QED
-
-Theorem compile_If:
-  ^(get_goal "loopLang$If")
-Proof
-  rpt strip_tac
-  \\ fs [loopSemTheory.evaluate_def]
-  \\ Cases_on ‘lookup r1 s.locals’ \\ fs []
-  \\ Cases_on ‘x’ \\ fs []
-  \\ Cases_on ‘get_var_imm ri s’ \\ fs []
-  \\ Cases_on ‘x’ \\ fs []
-  \\ fs [comp_def]
-  \\ rpt (pairarg_tac \\ fs [])
-  \\ fs [wordSemTheory.evaluate_def]
-  \\ pairarg_tac \\ fs []
-  \\ fs [get_var_def]
-  \\ Cases_on ‘lookup r1 t.locals’ \\ fs []
-  THEN1 (
-   rveq \\ fs []
-   \\ cheat
-   )
-  \\ Cases_on ‘x’ \\ fs []
-  THEN1 (
-   Cases_on ‘get_var_imm ri t’ \\ fs []
-   THEN1 (
-    rveq \\ fs []
-    \\ cheat
-    )
-   \\ cheat
-   )
-  \\ cheat
-
- (* \\ qabbrev_tac `resp = evaluate (if word_cmp cmp c c' then c1 else c2,s)`
-  \\ PairCases_on ‘resp’ \\ fs [cut_res_def]
-  \\ Cases_on ‘resp0 ≠ NONE’ \\ fs [] \\ rveq \\ fs []
-  THEN1 (
-   first_x_assum (qspecl_then [‘t’,‘ctxt’,‘retv’,‘l’] mp_tac)
-   \\ impl_tac \\ fs []
-   \\ fs [assigned_vars_def,no_Loops_def,no_Loop_def,every_prog_def]
-   \\ cheat
-   )
-   \\ cheat
-  *)
+  rpt strip_tac >>
+  fs [loopSemTheory.evaluate_def, comp_def, evaluate_def] >>
+  cases_on ‘lookup n s.locals’ >>
+  fs []  >> rveq >>
+  TOP_CASE_TAC >>
+  fs [find_var_def, locals_rel_def, get_var_def] >>
+  res_tac >> rveq >>
+  TOP_CASE_TAC >> fs [isWord_def] >>
+  fs [flush_state_def, state_rel_def,
+      loopSemTheory.call_env_def]
 QED
 
 Theorem compile_Seq:
   ^(get_goal "comp _ (loopLang$Seq _ _)")
 Proof
-  rpt strip_tac
-  \\ fs [loopSemTheory.evaluate_def]
-  \\ pairarg_tac \\ fs [comp_def]
-  \\ rpt (pairarg_tac \\ fs [])
-  \\ fs [wordSemTheory.evaluate_def]
-  \\ rpt (pairarg_tac \\ fs [])
-  \\ first_x_assum (qspecl_then [‘t’,‘ctxt’,‘retv’,‘l’] mp_tac)
-  \\ impl_tac THEN1
-   (fs [] \\ conj_tac THEN1 (CCONTR_TAC \\ fs [])
-    \\ fs [no_Loops_def,no_Loop_def,every_prog_def]
-    \\ qpat_x_assum ‘_ ⊆ domain ctxt’ mp_tac
-    \\ fs [assigned_vars_def]
-    \\ once_rewrite_tac [assigned_vars_acc] \\ fs [])
-  \\ fs [] \\ strip_tac
-  \\ reverse (Cases_on ‘res'’)
-  THEN1
-   (fs [] \\ rveq \\ fs [] \\ Cases_on ‘x’ \\ fs []
-    \\ IF_CASES_TAC \\ fs [])
-  \\ fs [] \\ rveq \\ fs []
-  \\ rename [‘state_rel s2 t2’]
-  \\ first_x_assum drule
-  \\ rpt (disch_then drule)
-  \\ disch_then (qspec_then ‘l'’ mp_tac)
-  \\ impl_tac THEN1
-   (qpat_x_assum ‘_ ⊆ domain ctxt’ mp_tac
-    \\ fs [no_Loops_def,no_Loop_def,every_prog_def]
-    \\ fs [assigned_vars_def]
-    \\ once_rewrite_tac [assigned_vars_acc] \\ fs [])
-  \\ fs [] \\ strip_tac \\ fs []
-  \\ Cases_on ‘res’ \\ fs []
-  \\ Cases_on ‘x’ \\ fs []
-QED
-
-Theorem lookup_not_NONE :
-  ∀ n locals. lookup n locals ≠ NONE ⇒ ∃ v. lookup n locals = SOME v
-Proof
-  rpt strip_tac
-  \\ rename [‘lookup n l’]
-  \\ Cases_on ‘l’ \\ fs [lookup_def,miscTheory.IS_SOME_EXISTS]
-  \\ fs [CaseEq "bool"]
-  \\ Cases_on ‘n’ \\ fs []
-  \\ metis_tac [miscTheory.IS_SOME_EXISTS,
-                quantHeuristicsTheory.IS_SOME_EQ_NOT_NONE]
-QED
-
-Theorem comp_exp_cc :
-! ctxt x s t. state_rel s t /\ locals_rel ctxt s.locals t.locals /\ eval s x <> NONE ⇒
-  word_exp t (comp_exp ctxt x) = eval s x
-Proof
-  ho_match_mp_tac comp_exp_ind \\ rw []
-  \\ fs [comp_exp_def,word_exp_def,eval_def]
-  THEN1 (
-   fs [find_var_def,locals_rel_def]
-   \\ drule lookup_not_NONE \\ rw []
-   \\ first_x_assum drule
-   \\ strip_tac \\ fs []
-   )
-  THEN1 (
-   fs [state_rel_def,globals_rel_def]
-   \\ Cases_on ‘FLOOKUP s.globals m’ \\ fs []
-   )
-  THEN1 (
-   Cases_on ‘eval s x’ \\ fs []
-   \\ Cases_on ‘x'’ \\ fs []
-   \\ first_x_assum drule \\ fs []
-   \\ strip_tac
-   \\ fs [state_rel_def,wordSemTheory.mem_load_def,
-          loopSemTheory.mem_load_def]
-   )
-  THEN1 (
-   Cases_on ‘eval s' x’ \\ fs []
-   \\ Cases_on ‘x'’ \\ fs []
-   \\ first_x_assum drule \\ fs []
-   )
-  \\ Cases_on ‘the_words (MAP (λa. eval s a) wexps)’ \\ fs []
-  \\ qsuff_tac ‘the_words (MAP (λa. word_exp t a) (MAP (λa. comp_exp ctxt a) wexps)) = SOME x’
-  THEN1 fs []
-  \\ pop_assum mp_tac
-  \\ pop_assum kall_tac
-  \\ rpt (pop_assum mp_tac)
-  \\ qid_spec_tac ‘x’
-  \\ qid_spec_tac ‘wexps’
-  \\ Induct \\ fs []
-  \\ fs [the_words_def,CaseEq"option",CaseEq"word_loc",
-         PULL_EXISTS,PULL_FORALL]
-  \\ rpt strip_tac
-  \\ first_x_assum (qspecl_then [‘h’,‘s’,‘t’] mp_tac)
-  \\ impl_tac \\ fs []
+  rpt strip_tac >>
+  fs [loopSemTheory.evaluate_def] >>
+  pairarg_tac >> fs [comp_def] >>
+  rpt (pairarg_tac >> fs []) >>
+  fs [evaluate_def] >>
+  rpt (pairarg_tac >> fs []) >>
+  first_x_assum (qspecl_then [‘t’,‘ctxt’,‘retv’,‘l’] mp_tac) >>
+  impl_tac
+  >- (
+   fs [] >>
+   conj_tac >- (CCONTR_TAC >> fs []) >>
+   fs [no_Loops_def, no_Loop_def, every_prog_def] >>
+   qpat_x_assum ‘_ ⊆ domain ctxt’ mp_tac >>
+   fs [assigned_vars_def] >>
+   once_rewrite_tac [assigned_vars_acc] >> fs []) >>
+  fs [] >> strip_tac >>
+  reverse (Cases_on ‘res'’) >> fs [] >> rveq >> fs []
+  >- (
+   Cases_on ‘x’ >> fs [] >>
+   IF_CASES_TAC >> fs []) >>
+  rename [‘state_rel s2 t2’] >>
+  first_x_assum drule >>
+  rpt (disch_then drule) >>
+  disch_then (qspec_then ‘l'’ mp_tac) >>
+  impl_tac
+  >- (
+   qpat_x_assum ‘_ ⊆ domain ctxt’ mp_tac >>
+   fs [no_Loops_def, no_Loop_def, every_prog_def] >>
+   fs [assigned_vars_def] >>
+   once_rewrite_tac [assigned_vars_acc] >> fs []) >>
+  fs [] >> strip_tac >> fs [] >>
+  Cases_on ‘res’ >> fs [] >>
+  Cases_on ‘x’ >> fs []
 QED
 
 Theorem compile_Assign:
   ^(get_goal "loopLang$Assign") ∧
   ^(get_goal "loopLang$LocValue")
 Proof
-  rpt strip_tac
-  \\ fs [loopSemTheory.evaluate_def,comp_def,
-         wordSemTheory.evaluate_def]
-  THEN1 (
-   Cases_on ‘eval s exp’ \\ fs []
-   \\ rveq \\ fs []
-   \\ drule comp_exp_cc
-   \\ disch_then drule
-   \\ disch_then (qspec_then ‘exp’ mp_tac)
-   \\ fs [loopSemTheory.set_var_def,wordSemTheory.set_var_def]
-   \\ strip_tac
-   \\ fs [state_rel_def]
-   \\ CONJ_TAC
-   THEN1 (
-    fs [lookup_insert,CaseEq "bool",assigned_vars_def]
-    \\ imp_res_tac find_var_neq_0 \\ fs []
-    )
-   \\ match_mp_tac locals_rel_insert
-   \\ fs [assigned_vars_def]
-   )
-  \\ fs [CaseEq "bool"]
-  \\ rveq \\ fs []
-  \\ fs [state_rel_def,loopSemTheory.set_var_def,
-         wordSemTheory.set_var_def]
-  \\ rpt strip_tac
-  THEN1 (
-   fs [code_rel_def,domain_lookup,EXISTS_PROD]
-   \\ metis_tac []
-   )
-  THEN1 (
-   fs [lookup_insert,CaseEq "bool",assigned_vars_def]
-   \\ imp_res_tac find_var_neq_0 \\ fs []
-   )
-  \\ match_mp_tac locals_rel_insert
-  \\ fs [assigned_vars_def]
+  rpt strip_tac >>
+  fs [loopSemTheory.evaluate_def,
+      comp_def, evaluate_def]
+  >- (
+   cases_on ‘eval s exp’ >> fs [] >>
+   rveq >> fs [] >>
+   imp_res_tac comp_exp_preserves_eval >>
+   fs [loopSemTheory.set_var_def, set_var_def] >>
+   conj_tac >- fs [state_rel_def] >>
+   conj_tac
+   >- (
+    fs [lookup_insert, CaseEq "bool", assigned_vars_def] >>
+    imp_res_tac find_var_neq_0 >> fs []) >>
+   match_mp_tac locals_rel_insert >>
+   fs [assigned_vars_def]) >>
+  fs [CaseEq "bool"] >> rveq >> fs [] >>
+  fs [loopSemTheory.set_var_def, set_var_def] >>
+  conj_tac
+  >- (
+   fs [state_rel_def,
+       code_rel_def,domain_lookup,EXISTS_PROD] >>
+   metis_tac []) >>
+  conj_tac >- fs [state_rel_def] >>
+  conj_tac
+  >- (
+   fs [lookup_insert, CaseEq "bool", assigned_vars_def] >>
+   imp_res_tac find_var_neq_0 >> fs []) >>
+  match_mp_tac locals_rel_insert >>
+  fs [assigned_vars_def]
 QED
 
 Theorem compile_Store:
   ^(get_goal "loopLang$Store") ∧
   ^(get_goal "loopLang$StoreByte")
 Proof
- cheat
+  rpt strip_tac >>
+  fs [loopSemTheory.evaluate_def,
+      comp_def, evaluate_def]
+  >- (
+   fs [CaseEq "option", CaseEq "word_loc"] >> rveq >>
+   imp_res_tac comp_exp_preserves_eval >>
+   fs [] >>
+   drule_all locals_rel_get_var >>
+   strip_tac >> fs [] >>
+   fs [loopSemTheory.mem_store_def, mem_store_def] >>
+   rveq >> fs [state_rel_def]) >>
+  fs [CaseEq "option", CaseEq "word_loc"] >> rveq >>
+  fs [inst_def, word_exp_def] >>
+  drule locals_rel_intro >>
+  strip_tac >>
+  res_tac >> fs [] >>
+  fs [find_var_def, the_words_def, word_op_def] >>
+  fs [get_var_def] >>
+  fs [state_rel_def]
 QED
 
 Theorem compile_LoadByte:
   ^(get_goal "loopLang$LoadByte")
 Proof
-  cheat
+  rpt strip_tac >>
+  fs [loopSemTheory.evaluate_def,
+      comp_def, evaluate_def] >>
+  fs [CaseEq "option", CaseEq "word_loc"] >> rveq >>
+  fs [inst_def, word_exp_def] >>
+  drule locals_rel_intro >>
+  strip_tac >>
+  res_tac >> fs [] >>
+  fs [find_var_def, the_words_def, word_op_def] >>
+  drule state_rel_intro >>
+  strip_tac >> fs [] >>
+  fs [loopSemTheory.set_var_def, set_var_def] >>
+  conj_tac >- fs [state_rel_def] >>
+  fs [assigned_vars_def] >>
+  imp_res_tac find_var_neq_0 >>
+  fs [domain_lookup, lookup_insert, CaseEq "bool"] >>
+  conj_tac
+  >- (CCONTR_TAC >> res_tac >> fs []) >>
+  drule locals_rel_insert >>
+  disch_then (qspecl_then [‘Word (w2w b)’, ‘v’] mp_tac) >>
+  fs [domain_lookup, find_var_def]
 QED
 
 Theorem compile_SetGlobal:
   ^(get_goal "loopLang$SetGlobal")
 Proof
-  cheat
+  rpt strip_tac >>
+  fs [loopSemTheory.evaluate_def,
+      comp_def, evaluate_def] >>
+  fs [CaseEq "option"] >>
+  rveq >> fs [] >>
+  imp_res_tac comp_exp_preserves_eval >>
+  fs [] >>
+  fs [state_rel_def, set_store_def,
+      loopSemTheory.set_globals_def, globals_rel_def] >>
+  rw [FLOOKUP_UPDATE]
 QED
 
 Theorem compile_FFI:
   ^(get_goal "loopLang$FFI")
 Proof
-  rpt strip_tac
-  \\ fs [loopSemTheory.evaluate_def]
-  \\ Cases_on ‘lookup len1 s.locals’ \\ fs []
-  \\ Cases_on ‘x’ \\ fs []
-  \\ Cases_on ‘lookup ptr1 s.locals’ \\ fs []
-  \\ Cases_on ‘x’ \\ fs []
-  \\ Cases_on ‘lookup len2 s.locals’ \\ fs []
-  \\ Cases_on ‘x’ \\ fs []
-  \\ Cases_on ‘lookup ptr2 s.locals’ \\ fs []
-  \\ Cases_on ‘x’ \\ fs []
-  \\ Cases_on ‘cut_state cutset s’ \\ fs []
-  \\ Cases_on ‘read_bytearray c' (w2n c)
-               (mem_load_byte_aux x.memory x.mdomain x.be)’ \\ fs []
-  \\ Cases_on ‘ read_bytearray c'³' (w2n c'')
-                (mem_load_byte_aux x.memory x.mdomain x.be)’ \\ fs []
-  \\ Cases_on ‘call_FFI x.ffi ffi_index x' x''’ \\ fs [comp_def,find_var_def]
-  THEN1 (
-   rveq \\ fs []
-   \\ fs [wordSemTheory.evaluate_def,get_var_def]
-   \\ cheat
-   )
-  \\ rveq \\ fs []
-  \\ fs [wordSemTheory.evaluate_def,get_var_def]
-  \\ cheat
+  rpt strip_tac >>
+  fs [loopSemTheory.evaluate_def,
+      comp_def, evaluate_def] >>
+  fs [CaseEq "option", CaseEq "word_loc"] >>
+  rveq >> fs [] >>
+  fs [find_var_def, get_var_def] >>
+  imp_res_tac state_rel_intro >>
+  imp_res_tac locals_rel_intro >>
+  res_tac >> fs [] >>
+  fs [loopSemTheory.cut_state_def] >> rveq >>
+  fs [cut_env_def] >>
+  ‘domain cutset ⊆ domain t.locals’ by cheat >>
+  fs [] >>
+  TOP_CASE_TAC >> fs [] >> rveq >> fs [] >>
+  fs [state_rel_def, flush_state_def,
+      loopSemTheory.call_env_def] >>
+  cheat
 QED
 
-Theorem locals_rel_get_var:
-  locals_rel ctxt l t.locals ∧ lookup n l = SOME w ⇒
-  wordSem$get_var (find_var ctxt n) t = SOME w
+
+Theorem compile_If:
+  ^(get_goal "loopLang$If")
 Proof
-  fs [locals_rel_def] \\ rw[] \\ res_tac
-  \\ fs [find_var_def,get_var_def]
+  rpt strip_tac
+  >> fs [loopSemTheory.evaluate_def]
+  >> Cases_on ‘lookup r1 s.locals’ >> fs []
+  >> Cases_on ‘x’ >> fs []
+  >> Cases_on ‘get_var_imm ri s’ >> fs []
+  >> Cases_on ‘x’ >> fs []
+  >> fs [comp_def]
+  >> rpt (pairarg_tac >> fs [])
+  >> fs [wordSemTheory.evaluate_def]
+  >> pairarg_tac >> fs []
+  >> fs [get_var_def]
+  >> Cases_on ‘lookup r1 t.locals’ >> fs []
+  >- (
+   rveq >> fs []
+   >> cheat
+   )
+  >> Cases_on ‘x’ >> fs []
+  >- (
+   Cases_on ‘get_var_imm ri t’ >> fs []
+   >- (
+    rveq >> fs []
+    >> cheat
+    )
+   >> cheat
+   )
+  >> cheat
+
+ (* >> qabbrev_tac `resp = evaluate (if word_cmp cmp c c' then c1 else c2,s)`
+  >> PairCases_on ‘resp’ >> fs [cut_res_def]
+  >> Cases_on ‘resp0 ≠ NONE’ >> fs [] >> rveq >> fs []
+  >- (
+   first_x_assum (qspecl_then [‘t’,‘ctxt’,‘retv’,‘l’] mp_tac)
+   >> impl_tac >> fs []
+   >> fs [assigned_vars_def,no_Loops_def,no_Loop_def,every_prog_def]
+   >> cheat
+   )
+   >> cheat
+  *)
 QED
+
+
 
 Theorem locals_rel_get_vars:
   ∀argvars argvals.
@@ -559,24 +619,24 @@ Theorem locals_rel_get_vars:
     wordSem$get_vars (MAP (find_var ctxt) argvars) t = SOME argvals ∧
     LENGTH argvals = LENGTH argvars
 Proof
-  Induct \\ fs [loopSemTheory.get_vars_def,get_vars_def,CaseEq"option"]
-  \\ rw [] \\ imp_res_tac locals_rel_get_var \\ fs []
+  Induct >> fs [loopSemTheory.get_vars_def,get_vars_def,CaseEq"option"]
+  >> rw [] >> imp_res_tac locals_rel_get_var >> fs []
 QED
 
 Theorem compile_Raise:
   ^(get_goal "loopLang$Raise")
 Proof
   fs [comp_def,loopSemTheory.evaluate_def,CaseEq"option"]
-  \\ rw [] \\ fs [evaluate_def]
-  \\ imp_res_tac locals_rel_get_var \\ fs []
-  \\ Cases_on ‘jump_exc t’ \\ fs []
-  THEN1 (fs [jump_exc_def,state_rel_def,loopSemTheory.call_env_def])
-  \\ fs [CaseEq"prod",PULL_EXISTS]
-  \\ PairCases_on ‘x’ \\ fs [loopSemTheory.call_env_def]
-  \\ pop_assum mp_tac
-  \\ fs [CaseEq"option",CaseEq"prod",jump_exc_def,CaseEq"stack_frame",CaseEq"list"]
-  \\ strip_tac \\ fs [] \\ rveq \\ fs []
-  \\ fs [state_rel_def]
+  >> rw [] >> fs [evaluate_def]
+  >> imp_res_tac locals_rel_get_var >> fs []
+  >> Cases_on ‘jump_exc t’ >> fs []
+  >- (fs [jump_exc_def,state_rel_def,loopSemTheory.call_env_def])
+  >> fs [CaseEq"prod",PULL_EXISTS]
+  >> PairCases_on ‘x’ >> fs [loopSemTheory.call_env_def]
+  >> pop_assum mp_tac
+  >> fs [CaseEq"option",CaseEq"prod",jump_exc_def,CaseEq"stack_frame",CaseEq"list"]
+  >> strip_tac >> fs [] >> rveq >> fs []
+  >> fs [state_rel_def]
 QED
 
 Triviality state_rel_IMP:
@@ -594,13 +654,13 @@ QED
 Theorem domain_toNumSet:
   domain (toNumSet ps) = set ps
 Proof
-  Induct_on ‘ps’ \\ fs [toNumSet_def]
+  Induct_on ‘ps’ >> fs [toNumSet_def]
 QED
 
 Theorem domain_make_ctxt:
   ∀n ps l. domain (make_ctxt n ps l) = domain l UNION set ps
 Proof
-  Induct_on ‘ps’ \\ fs [make_ctxt_def] \\ fs [EXTENSION] \\ metis_tac []
+  Induct_on ‘ps’ >> fs [make_ctxt_def] >> fs [EXTENSION] >> metis_tac []
 QED
 
 Theorem make_ctxt_inj:
@@ -608,12 +668,12 @@ Theorem make_ctxt_inj:
            (∀x y v. lookup x (make_ctxt n xs l) = SOME v ∧
                     lookup y (make_ctxt n xs l) = SOME v ⇒ x = y)
 Proof
-  Induct_on ‘xs’ \\ fs [make_ctxt_def] \\ rw []
-  \\ first_x_assum (qspecl_then [‘insert h n l’,‘n+2’] mp_tac)
-  \\ impl_tac THEN1
-   (fs [lookup_insert] \\ rw []
-    \\ CCONTR_TAC \\ fs [] \\ res_tac \\ fs [])
-  \\ metis_tac []
+  Induct_on ‘xs’ >> fs [make_ctxt_def] >> rw []
+  >> first_x_assum (qspecl_then [‘insert h n l’,‘n+2’] mp_tac)
+  >> impl_tac >-
+   (fs [lookup_insert] >> rw []
+    >> CCONTR_TAC >> fs [] >> res_tac >> fs [])
+  >> metis_tac []
 QED
 
 Triviality make_ctxt_APPEND:
@@ -621,13 +681,13 @@ Triviality make_ctxt_APPEND:
     make_ctxt n (xs ++ ys) l =
     make_ctxt (n + 2 * LENGTH xs) ys (make_ctxt n xs l)
 Proof
-  Induct \\ fs [make_ctxt_def,MULT_CLAUSES]
+  Induct >> fs [make_ctxt_def,MULT_CLAUSES]
 QED
 
 Triviality make_ctxt_NOT_MEM:
   ∀xs n l x. ~MEM x xs ⇒ lookup x (make_ctxt n xs l) = lookup x l
 Proof
-  Induct \\ fs [make_ctxt_def,lookup_insert]
+  Induct >> fs [make_ctxt_def,lookup_insert]
 QED
 
 Theorem lookup_EL_make_ctxt:
@@ -635,7 +695,7 @@ Theorem lookup_EL_make_ctxt:
     k < LENGTH params ∧ ALL_DISTINCT params ⇒
     lookup (EL k params) (make_ctxt n params l) = SOME (2 * k + n)
 Proof
-  Induct \\ Cases_on ‘k’ \\ fs [] \\ fs [make_ctxt_def,make_ctxt_NOT_MEM]
+  Induct >> Cases_on ‘k’ >> fs [] >> fs [make_ctxt_def,make_ctxt_NOT_MEM]
 QED
 
 Theorem lookup_make_ctxt_range:
@@ -643,9 +703,9 @@ Theorem lookup_make_ctxt_range:
     lookup n (make_ctxt m xs l) = SOME y ⇒
     lookup n l = SOME y ∨ m ≤ y
 Proof
-  Induct \\ fs [make_ctxt_def] \\ rw []
-  \\ first_x_assum drule
-  \\ fs [lookup_insert] \\ rw [] \\ fs []
+  Induct >> fs [make_ctxt_def] >> rw []
+  >> first_x_assum drule
+  >> fs [lookup_insert] >> rw [] >> fs []
 QED
 
 Theorem locals_rel_make_ctxt:
@@ -654,27 +714,27 @@ Theorem locals_rel_make_ctxt:
   locals_rel (make_ctxt 2 (params ++ xs) LN)
     (fromAList (ZIP (params,l))) (fromList2 (retv::l))
 Proof
-  fs [locals_rel_def] \\ rw []
-  THEN1
-   (fs [INJ_DEF,find_var_def,domain_lookup] \\ rw [] \\ rfs []
-    \\ rveq \\ fs []
-    \\ imp_res_tac (MP_CANON make_ctxt_inj) \\ fs [lookup_def])
-  THEN1
-   (Cases_on ‘lookup n (make_ctxt 2 (params ++ xs) LN)’ \\ simp []
-    \\ drule lookup_make_ctxt_range \\ fs [lookup_def])
-  \\ fs [lookup_fromAList]
-  \\ imp_res_tac ALOOKUP_MEM
-  \\ rfs [MEM_ZIP]  \\ rveq \\ fs [make_ctxt_APPEND]
-  \\ rename [‘k < LENGTH _’]
-  \\ ‘k < LENGTH params’ by fs []
-  \\ drule EL_MEM \\ strip_tac
-  \\ ‘~MEM (EL k params) xs’ by (fs [IN_DISJOINT] \\ metis_tac [])
-  \\ fs [make_ctxt_NOT_MEM]
-  \\ fs [lookup_EL_make_ctxt]
-  \\ fs [lookup_fromList2,EVEN_ADD,EVEN_DOUBLE]
-  \\ ‘2 * k + 2 = (SUC k) * 2’ by fs []
-  \\ asm_rewrite_tac [MATCH_MP MULT_DIV (DECIDE “0 < 2:num”)]
-  \\ fs [lookup_fromList]
+  fs [locals_rel_def] >> rw []
+  >-
+   (fs [INJ_DEF,find_var_def,domain_lookup] >> rw [] >> rfs []
+    >> rveq >> fs []
+    >> imp_res_tac (MP_CANON make_ctxt_inj) >> fs [lookup_def])
+  >-
+   (Cases_on ‘lookup n (make_ctxt 2 (params ++ xs) LN)’ >> simp []
+    >> drule lookup_make_ctxt_range >> fs [lookup_def])
+  >> fs [lookup_fromAList]
+  >> imp_res_tac ALOOKUP_MEM
+  >> rfs [MEM_ZIP]  >> rveq >> fs [make_ctxt_APPEND]
+  >> rename [‘k < LENGTH _’]
+  >> ‘k < LENGTH params’ by fs []
+  >> drule EL_MEM >> strip_tac
+  >> ‘~MEM (EL k params) xs’ by (fs [IN_DISJOINT] >> metis_tac [])
+  >> fs [make_ctxt_NOT_MEM]
+  >> fs [lookup_EL_make_ctxt]
+  >> fs [lookup_fromList2,EVEN_ADD,EVEN_DOUBLE]
+  >> ‘2 * k + 2 = (SUC k) * 2’ by fs []
+  >> asm_rewrite_tac [MATCH_MP MULT_DIV (DECIDE “0 < 2:num”)]
+  >> fs [lookup_fromList]
 QED
 
 Theorem domain_mk_new_cutset_not_empty:
@@ -688,13 +748,13 @@ Theorem cut_env_mk_new_cutset:
   ∃env1. cut_env (mk_new_cutset ctxt x1) l2 = SOME env1 ∧
          locals_rel ctxt (inter l1 x1) env1
 Proof
-  fs [locals_rel_def,SUBSET_DEF,cut_env_def] \\ fs [lookup_inter_alt]
-  \\ fs [mk_new_cutset_def,domain_toNumSet,MEM_MAP,set_fromNumSet,PULL_EXISTS]
-  \\ fs [DISJ_IMP_THM,PULL_EXISTS]
-  \\ strip_tac \\ fs [domain_lookup]
-  \\ rw [] \\ res_tac \\ fs [] \\ rveq \\ fs [find_var_def]
-  \\ rw [] \\ res_tac \\ fs [] \\ rveq \\ fs [find_var_def]
-  \\ disj2_tac \\ qexists_tac ‘n’ \\ fs []
+  fs [locals_rel_def,SUBSET_DEF,cut_env_def] >> fs [lookup_inter_alt]
+  >> fs [mk_new_cutset_def,domain_toNumSet,MEM_MAP,set_fromNumSet,PULL_EXISTS]
+  >> fs [DISJ_IMP_THM,PULL_EXISTS]
+  >> strip_tac >> fs [domain_lookup]
+  >> rw [] >> res_tac >> fs [] >> rveq >> fs [find_var_def]
+  >> rw [] >> res_tac >> fs [] >> rveq >> fs [find_var_def]
+  >> disj2_tac >> qexists_tac ‘n’ >> fs []
 QED
 
 Theorem env_to_list_IMP:
@@ -702,17 +762,17 @@ Theorem env_to_list_IMP:
   domain (fromAList l) = domain env1 ∧
   ∀x. lookup x (fromAList l) = lookup x env1
 Proof
-  strip_tac \\ drule env_to_list_lookup_equiv
-  \\ fs [EXTENSION,domain_lookup,lookup_fromAList]
+  strip_tac >> drule env_to_list_lookup_equiv
+  >> fs [EXTENSION,domain_lookup,lookup_fromAList]
 QED
 
 Theorem cut_env_mk_new_cutset_IMP:
   cut_env (mk_new_cutset ctxt x1) l1 = SOME l2 ⇒
   lookup 0 l2 = lookup 0 l1
 Proof
-  fs [cut_env_def] \\ rw []
-  \\ fs [SUBSET_DEF,mk_new_cutset_def]
-  \\ fs [lookup_inter_alt]
+  fs [cut_env_def] >> rw []
+  >> fs [SUBSET_DEF,mk_new_cutset_def]
+  >> fs [lookup_inter_alt]
 QED
 
 Triviality LASTN_ADD_CONS:
@@ -724,314 +784,314 @@ QED
 Theorem compile_Call:
   ^(get_goal "comp _ (loopLang$Call _ _ _ _)")
 Proof
-  rw [] \\ qpat_x_assum ‘evaluate _ = (res,_)’ mp_tac
-  \\ simp [loopSemTheory.evaluate_def]
-  \\ simp [CaseEq"option"]
-  \\ strip_tac \\ fs []
-  \\ rename [‘find_code _ _ _ = SOME x’]
-  \\ PairCases_on ‘x’ \\ fs []
-  \\ rename [‘find_code _ _ _ = SOME (new_env,new_code)’]
-  \\ ‘~bad_dest_args dest (MAP (find_var ctxt) argvars)’ by
-       (pop_assum kall_tac \\ Cases_on ‘dest’ \\ fs [bad_dest_args_def]
-        \\ fs [loopSemTheory.find_code_def]
-        \\ imp_res_tac locals_rel_get_vars \\ CCONTR_TAC \\ fs [])
-  \\ Cases_on ‘ret’ \\ fs []
-  THEN1
+  rw [] >> qpat_x_assum ‘evaluate _ = (res,_)’ mp_tac
+  >> simp [loopSemTheory.evaluate_def]
+  >> simp [CaseEq"option"]
+  >> strip_tac >> fs []
+  >> rename [‘find_code _ _ _ = SOME x’]
+  >> PairCases_on ‘x’ >> fs []
+  >> rename [‘find_code _ _ _ = SOME (new_env,new_code)’]
+  >> ‘~bad_dest_args dest (MAP (find_var ctxt) argvars)’ by
+       (pop_assum kall_tac >> Cases_on ‘dest’ >> fs [bad_dest_args_def]
+        >> fs [loopSemTheory.find_code_def]
+        >> imp_res_tac locals_rel_get_vars >> CCONTR_TAC >> fs [])
+  >> Cases_on ‘ret’ >> fs []
+  >-
    (fs [comp_def,evaluate_def]
-    \\ imp_res_tac locals_rel_get_vars \\ fs [add_ret_loc_def]
-    \\ fs [get_vars_def,get_var_def]
-    \\ simp [bad_dest_args_def,call_env_def,dec_clock_def]
-    \\ ‘∃args1 prog1 ss1 name1 ctxt1 l1.
+    >> imp_res_tac locals_rel_get_vars >> fs [add_ret_loc_def]
+    >> fs [get_vars_def,get_var_def]
+    >> simp [bad_dest_args_def,call_env_def,dec_clock_def]
+    >> ‘∃args1 prog1 ss1 name1 ctxt1 l1.
          find_code dest (retv::argvals) t.code t.stack_size = SOME (args1,prog1,ss1) ∧
          FST (comp ctxt1 new_code l1) = prog1 ∧
          lookup 0 (fromList2 args1) = SOME retv ∧
          locals_rel ctxt1 new_env (fromList2 args1) ∧ no_Loops new_code ∧
          domain (assigned_vars new_code LN) ⊆ domain ctxt1’ by
       (qpat_x_assum ‘_ = (res,_)’ kall_tac
-       \\ Cases_on ‘dest’ \\ fs [loopSemTheory.find_code_def]
-       THEN1
+       >> Cases_on ‘dest’ >> fs [loopSemTheory.find_code_def]
+       >-
         (fs [CaseEq"word_loc",CaseEq"num",CaseEq"option",CaseEq"prod",CaseEq"bool"]
-         \\ rveq \\ fs [code_rel_def,state_rel_def]
-         \\ first_x_assum drule \\ strip_tac \\ fs []
-         \\ fs [find_code_def]
-         \\ ‘∃x l. argvals = SNOC x l’ by metis_tac [SNOC_CASES]
-         \\ qpat_x_assum ‘_ = Loc loc 0’ mp_tac
-         \\ rveq \\ rewrite_tac [GSYM SNOC,LAST_SNOC,FRONT_SNOC] \\ fs []
-         \\ strip_tac \\ rveq \\ fs []
-         \\ simp [compile_def]
-         \\ qmatch_goalsub_abbrev_tac ‘comp ctxt2 _ ll2’
-         \\ qexists_tac ‘ctxt2’ \\ qexists_tac ‘ll2’ \\ fs []
-         \\ conj_tac THEN1 fs [lookup_fromList2,lookup_fromList]
-         \\ simp [Abbr‘ctxt2’,domain_make_ctxt,set_fromNumSet,
+         >> rveq >> fs [code_rel_def,state_rel_def]
+         >> first_x_assum drule >> strip_tac >> fs []
+         >> fs [find_code_def]
+         >> ‘∃x l. argvals = SNOC x l’ by metis_tac [SNOC_CASES]
+         >> qpat_x_assum ‘_ = Loc loc 0’ mp_tac
+         >> rveq >> rewrite_tac [GSYM SNOC,LAST_SNOC,FRONT_SNOC] >> fs []
+         >> strip_tac >> rveq >> fs []
+         >> simp [compile_def]
+         >> qmatch_goalsub_abbrev_tac ‘comp ctxt2 _ ll2’
+         >> qexists_tac ‘ctxt2’ >> qexists_tac ‘ll2’ >> fs []
+         >> conj_tac >- fs [lookup_fromList2,lookup_fromList]
+         >> simp [Abbr‘ctxt2’,domain_make_ctxt,set_fromNumSet,
                   domain_difference,domain_toNumSet]
-         \\ reverse conj_tac THEN1 fs [SUBSET_DEF]
-         \\ match_mp_tac locals_rel_make_ctxt
-         \\ fs [IN_DISJOINT,set_fromNumSet,domain_difference,
+         >> reverse conj_tac >- fs [SUBSET_DEF]
+         >> match_mp_tac locals_rel_make_ctxt
+         >> fs [IN_DISJOINT,set_fromNumSet,domain_difference,
                 domain_toNumSet,GSYM IMP_DISJ_THM])
-       \\ fs [CaseEq"word_loc",CaseEq"num",CaseEq"option",CaseEq"prod",CaseEq"bool"]
-       \\ rveq \\ fs [code_rel_def,state_rel_def]
-       \\ first_x_assum drule \\ strip_tac \\ fs []
-       \\ fs [find_code_def]
-       \\ simp [compile_def]
-       \\ qmatch_goalsub_abbrev_tac ‘comp ctxt2 _ ll2’
-       \\ qexists_tac ‘ctxt2’ \\ qexists_tac ‘ll2’ \\ fs []
-       \\ conj_tac THEN1 fs [lookup_fromList2,lookup_fromList]
-       \\ simp [Abbr‘ctxt2’,domain_make_ctxt,set_fromNumSet,
+       >> fs [CaseEq"word_loc",CaseEq"num",CaseEq"option",CaseEq"prod",CaseEq"bool"]
+       >> rveq >> fs [code_rel_def,state_rel_def]
+       >> first_x_assum drule >> strip_tac >> fs []
+       >> fs [find_code_def]
+       >> simp [compile_def]
+       >> qmatch_goalsub_abbrev_tac ‘comp ctxt2 _ ll2’
+       >> qexists_tac ‘ctxt2’ >> qexists_tac ‘ll2’ >> fs []
+       >> conj_tac >- fs [lookup_fromList2,lookup_fromList]
+       >> simp [Abbr‘ctxt2’,domain_make_ctxt,set_fromNumSet,
                 domain_difference,domain_toNumSet]
-       \\ reverse conj_tac THEN1 fs [SUBSET_DEF]
-       \\ match_mp_tac locals_rel_make_ctxt
-       \\ fs [IN_DISJOINT,set_fromNumSet,domain_difference,
+       >> reverse conj_tac >- fs [SUBSET_DEF]
+       >> match_mp_tac locals_rel_make_ctxt
+       >> fs [IN_DISJOINT,set_fromNumSet,domain_difference,
               domain_toNumSet,GSYM IMP_DISJ_THM])
-    \\ fs [] \\ imp_res_tac state_rel_IMP
-    \\ fs [] \\ IF_CASES_TAC \\ fs []
-    THEN1
-     (fs [CaseEq"bool"] \\ rveq \\ fs []
-      \\ fs [state_rel_def,flush_state_def])
-    \\ Cases_on ‘handler = NONE’ \\ fs [] \\ rveq
-    \\ Cases_on ‘evaluate (new_code,dec_clock s with locals := new_env)’ \\ fs []
-    \\ Cases_on ‘q’ \\ fs []
-    \\ Cases_on ‘x = Error’ \\ rveq \\ fs []
-    \\ qmatch_goalsub_abbrev_tac ‘wordSem$evaluate (_,tt)’
-    \\ first_x_assum (qspecl_then [‘tt’,‘ctxt1’,‘retv’,‘l1’] mp_tac)
-    \\ impl_tac
-    THEN1 (fs [Abbr‘tt’] \\ fs [state_rel_def,loopSemTheory.dec_clock_def])
-    \\ strip_tac \\ fs []
-    \\ Cases_on ‘x’ \\ fs [] \\ rveq \\ fs []
-    THEN1 fs [Abbr‘tt’]
-    \\ qexists_tac ‘t1’ \\ fs []
-    \\ qexists_tac ‘res1’ \\ fs []
-    \\ conj_tac THEN1 (Cases_on ‘res1’ \\ simp [CaseEq"option"] \\ fs [])
-    \\ rpt gen_tac \\ strip_tac \\ pop_assum mp_tac
-    \\ qunabbrev_tac ‘tt’ \\ fs [])
-  \\ fs [comp_def,evaluate_def]
-  \\ imp_res_tac locals_rel_get_vars \\ fs [add_ret_loc_def]
-  \\ fs [get_vars_def,get_var_def]
-  \\ simp [bad_dest_args_def,call_env_def,dec_clock_def]
-  \\ PairCases_on ‘x’ \\ PairCases_on ‘l’
-  \\ fs [] \\ imp_res_tac state_rel_IMP
-  \\ ‘∃args1 prog1 ss1 name1 ctxt1 l2.
+    >> fs [] >> imp_res_tac state_rel_IMP
+    >> fs [] >> IF_CASES_TAC >> fs []
+    >-
+     (fs [CaseEq"bool"] >> rveq >> fs []
+      >> fs [state_rel_def,flush_state_def])
+    >> Cases_on ‘handler = NONE’ >> fs [] >> rveq
+    >> Cases_on ‘evaluate (new_code,dec_clock s with locals := new_env)’ >> fs []
+    >> Cases_on ‘q’ >> fs []
+    >> Cases_on ‘x = Error’ >> rveq >> fs []
+    >> qmatch_goalsub_abbrev_tac ‘wordSem$evaluate (_,tt)’
+    >> first_x_assum (qspecl_then [‘tt’,‘ctxt1’,‘retv’,‘l1’] mp_tac)
+    >> impl_tac
+    >- (fs [Abbr‘tt’] >> fs [state_rel_def,loopSemTheory.dec_clock_def])
+    >> strip_tac >> fs []
+    >> Cases_on ‘x’ >> fs [] >> rveq >> fs []
+    >- fs [Abbr‘tt’]
+    >> qexists_tac ‘t1’ >> fs []
+    >> qexists_tac ‘res1’ >> fs []
+    >> conj_tac >- (Cases_on ‘res1’ >> simp [CaseEq"option"] >> fs [])
+    >> rpt gen_tac >> strip_tac >> pop_assum mp_tac
+    >> qunabbrev_tac ‘tt’ >> fs [])
+  >> fs [comp_def,evaluate_def]
+  >> imp_res_tac locals_rel_get_vars >> fs [add_ret_loc_def]
+  >> fs [get_vars_def,get_var_def]
+  >> simp [bad_dest_args_def,call_env_def,dec_clock_def]
+  >> PairCases_on ‘x’ >> PairCases_on ‘l’
+  >> fs [] >> imp_res_tac state_rel_IMP
+  >> ‘∃args1 prog1 ss1 name1 ctxt1 l2.
          find_code dest (Loc l0 l1::argvals) t.code t.stack_size = SOME (args1,prog1,ss1) ∧
          FST (comp ctxt1 new_code l2) = prog1 ∧
          lookup 0 (fromList2 args1) = SOME (Loc l0 l1) ∧
          locals_rel ctxt1 new_env (fromList2 args1) ∧ no_Loops new_code ∧
          domain (assigned_vars new_code LN) ⊆ domain ctxt1’ by
     (qpat_x_assum ‘_ = (res,_)’ kall_tac
-     \\ rpt (qpat_x_assum ‘∀x. _’ kall_tac)
-     \\ Cases_on ‘dest’ \\ fs [loopSemTheory.find_code_def]
-     THEN1
+     >> rpt (qpat_x_assum ‘∀x. _’ kall_tac)
+     >> Cases_on ‘dest’ >> fs [loopSemTheory.find_code_def]
+     >-
       (fs [CaseEq"word_loc",CaseEq"num",CaseEq"option",CaseEq"prod",CaseEq"bool"]
-       \\ rveq \\ fs [code_rel_def,state_rel_def]
-       \\ first_x_assum drule \\ strip_tac \\ fs []
-       \\ fs [find_code_def]
-       \\ ‘∃x l. argvals = SNOC x l’ by metis_tac [SNOC_CASES]
-       \\ qpat_x_assum ‘_ = Loc loc 0’ mp_tac
-       \\ rveq \\ rewrite_tac [GSYM SNOC,LAST_SNOC,FRONT_SNOC] \\ fs []
-       \\ strip_tac \\ rveq \\ fs []
-       \\ simp [compile_def]
-       \\ qmatch_goalsub_abbrev_tac ‘comp ctxt2 _ ll2’
-       \\ qexists_tac ‘ctxt2’ \\ qexists_tac ‘ll2’ \\ fs []
-       \\ conj_tac THEN1 fs [lookup_fromList2,lookup_fromList]
-       \\ simp [Abbr‘ctxt2’,domain_make_ctxt,set_fromNumSet,
+       >> rveq >> fs [code_rel_def,state_rel_def]
+       >> first_x_assum drule >> strip_tac >> fs []
+       >> fs [find_code_def]
+       >> ‘∃x l. argvals = SNOC x l’ by metis_tac [SNOC_CASES]
+       >> qpat_x_assum ‘_ = Loc loc 0’ mp_tac
+       >> rveq >> rewrite_tac [GSYM SNOC,LAST_SNOC,FRONT_SNOC] >> fs []
+       >> strip_tac >> rveq >> fs []
+       >> simp [compile_def]
+       >> qmatch_goalsub_abbrev_tac ‘comp ctxt2 _ ll2’
+       >> qexists_tac ‘ctxt2’ >> qexists_tac ‘ll2’ >> fs []
+       >> conj_tac >- fs [lookup_fromList2,lookup_fromList]
+       >> simp [Abbr‘ctxt2’,domain_make_ctxt,set_fromNumSet,
                 domain_difference,domain_toNumSet]
-       \\ reverse conj_tac THEN1 fs [SUBSET_DEF]
-       \\ match_mp_tac locals_rel_make_ctxt
-       \\ fs [IN_DISJOINT,set_fromNumSet,domain_difference,
+       >> reverse conj_tac >- fs [SUBSET_DEF]
+       >> match_mp_tac locals_rel_make_ctxt
+       >> fs [IN_DISJOINT,set_fromNumSet,domain_difference,
               domain_toNumSet,GSYM IMP_DISJ_THM])
-     \\ fs [CaseEq"word_loc",CaseEq"num",CaseEq"option",CaseEq"prod",CaseEq"bool"]
-     \\ rveq \\ fs [code_rel_def,state_rel_def]
-     \\ first_x_assum drule \\ strip_tac \\ fs []
-     \\ fs [find_code_def]
-     \\ simp [compile_def]
-     \\ qmatch_goalsub_abbrev_tac ‘comp ctxt2 _ ll2’
-     \\ qexists_tac ‘ctxt2’ \\ qexists_tac ‘ll2’ \\ fs []
-     \\ conj_tac THEN1 fs [lookup_fromList2,lookup_fromList]
-     \\ simp [Abbr‘ctxt2’,domain_make_ctxt,set_fromNumSet,
+     >> fs [CaseEq"word_loc",CaseEq"num",CaseEq"option",CaseEq"prod",CaseEq"bool"]
+     >> rveq >> fs [code_rel_def,state_rel_def]
+     >> first_x_assum drule >> strip_tac >> fs []
+     >> fs [find_code_def]
+     >> simp [compile_def]
+     >> qmatch_goalsub_abbrev_tac ‘comp ctxt2 _ ll2’
+     >> qexists_tac ‘ctxt2’ >> qexists_tac ‘ll2’ >> fs []
+     >> conj_tac >- fs [lookup_fromList2,lookup_fromList]
+     >> simp [Abbr‘ctxt2’,domain_make_ctxt,set_fromNumSet,
               domain_difference,domain_toNumSet]
-     \\ reverse conj_tac THEN1 fs [SUBSET_DEF]
-     \\ match_mp_tac locals_rel_make_ctxt
-     \\ fs [IN_DISJOINT,set_fromNumSet,domain_difference,
+     >> reverse conj_tac >- fs [SUBSET_DEF]
+     >> match_mp_tac locals_rel_make_ctxt
+     >> fs [IN_DISJOINT,set_fromNumSet,domain_difference,
             domain_toNumSet,GSYM IMP_DISJ_THM])
-  \\ Cases_on ‘handler’ \\ fs []
-  THEN1
+  >> Cases_on ‘handler’ >> fs []
+  >-
    (fs [evaluate_def,add_ret_loc_def,domain_mk_new_cutset_not_empty,cut_res_def]
-    \\ fs [loopSemTheory.cut_state_def]
-    \\ Cases_on ‘domain x1 ⊆ domain s.locals’ \\ fs []
-    \\ qpat_x_assum ‘locals_rel _ s.locals _’ assume_tac
-    \\ drule cut_env_mk_new_cutset
-    \\ rpt (disch_then drule) \\ strip_tac \\ fs []
-    \\ (IF_CASES_TAC \\ fs [] THEN1 (rveq \\ fs [flush_state_def,state_rel_def]))
-    \\ fs [CaseEq"prod",CaseEq"option"] \\ fs [] \\ rveq \\ fs []
-    \\ rename [‘_ = (SOME res2,st)’]
-    \\ qmatch_goalsub_abbrev_tac ‘wordSem$evaluate (_,tt)’
-    \\ fs [PULL_EXISTS]
-    \\ Cases_on ‘res2 = Error’ \\ fs []
-    \\ first_x_assum (qspecl_then [‘tt’,‘ctxt1’,‘Loc l0 l1’,‘l2’] mp_tac)
-    \\ (impl_tac THEN1
+    >> fs [loopSemTheory.cut_state_def]
+    >> Cases_on ‘domain x1 ⊆ domain s.locals’ >> fs []
+    >> qpat_x_assum ‘locals_rel _ s.locals _’ assume_tac
+    >> drule cut_env_mk_new_cutset
+    >> rpt (disch_then drule) >> strip_tac >> fs []
+    >> (IF_CASES_TAC >> fs [] >- (rveq >> fs [flush_state_def,state_rel_def]))
+    >> fs [CaseEq"prod",CaseEq"option"] >> fs [] >> rveq >> fs []
+    >> rename [‘_ = (SOME res2,st)’]
+    >> qmatch_goalsub_abbrev_tac ‘wordSem$evaluate (_,tt)’
+    >> fs [PULL_EXISTS]
+    >> Cases_on ‘res2 = Error’ >> fs []
+    >> first_x_assum (qspecl_then [‘tt’,‘ctxt1’,‘Loc l0 l1’,‘l2’] mp_tac)
+    >> (impl_tac >-
          (fs [Abbr‘tt’,call_env_def,push_env_def,isWord_def]
-          \\ pairarg_tac \\ fs [dec_clock_def,loopSemTheory.dec_clock_def,state_rel_def]))
-    \\ strip_tac \\ fs []
-    \\ Cases_on ‘res2’ \\ fs [] \\ rveq \\ fs []
-    THEN1
+          >> pairarg_tac >> fs [dec_clock_def,loopSemTheory.dec_clock_def,state_rel_def]))
+    >> strip_tac >> fs []
+    >> Cases_on ‘res2’ >> fs [] >> rveq >> fs []
+    >-
      (fs [Abbr‘tt’,call_env_def,push_env_def,dec_clock_def]
-      \\ pairarg_tac \\ fs [pop_env_def,set_var_def]
-      \\ imp_res_tac env_to_list_IMP
-      \\ fs [loopSemTheory.set_var_def,loopSemTheory.dec_clock_def]
-      \\ fs [state_rel_def]
-      \\ rename [‘find_var ctxt var_name’]
-      \\ ‘var_name IN domain ctxt’ by fs [assigned_vars_def]
-      \\ simp [lookup_insert]
-      \\ imp_res_tac find_var_neq_0 \\ fs []
-      \\ imp_res_tac cut_env_mk_new_cutset_IMP \\ fs []
-      \\ match_mp_tac locals_rel_insert \\ fs []
-      \\ fs [locals_rel_def])
-    \\ qunabbrev_tac ‘tt’
-    \\ pop_assum mp_tac
-    \\ Cases_on ‘res1’ THEN1 fs []
-    \\ disch_then (fn th => assume_tac (REWRITE_RULE [IMP_DISJ_THM] th))
-    \\ fs [] \\ Cases_on ‘x’ \\ fs []
-    \\ fs [state_rel_def]
-    \\ fs [call_env_def,push_env_def] \\ pairarg_tac \\ fs [dec_clock_def]
-    \\ fs [jump_exc_def,NOT_LESS]
-    \\ Cases_on ‘LENGTH t.stack <= t.handler’ \\ fs [LASTN_ADD_CONS]
-    \\ simp [CaseEq"option",CaseEq"prod",CaseEq"bool",set_var_def,CaseEq"list",
-             CaseEq"stack_frame"] \\ rw [] \\ fs [])
-  \\ PairCases_on ‘x’ \\ fs []
-  \\ rpt (pairarg_tac \\ fs [])
-  \\ fs [evaluate_def,add_ret_loc_def,domain_mk_new_cutset_not_empty,cut_res_def]
-  \\ fs [loopSemTheory.cut_state_def]
-  \\ Cases_on ‘domain x1 ⊆ domain s.locals’ \\ fs []
-  \\ qpat_x_assum ‘locals_rel _ s.locals _’ assume_tac
-  \\ drule cut_env_mk_new_cutset
-  \\ rpt (disch_then drule) \\ strip_tac \\ fs []
-  \\ (IF_CASES_TAC \\ fs [] THEN1 (rveq \\ fs [flush_state_def,state_rel_def]))
-  \\ fs [CaseEq"prod",CaseEq"option"] \\ fs [] \\ rveq \\ fs []
-  \\ rename [‘_ = (SOME res2,st)’]
-  \\ qmatch_goalsub_abbrev_tac ‘wordSem$evaluate (_,tt)’
-  \\ fs [PULL_EXISTS]
-  \\ Cases_on ‘res2 = Error’ \\ fs []
-  \\ first_x_assum (qspecl_then [‘tt’,‘ctxt1’,‘Loc l0 l1’,‘l2’] mp_tac)
-  \\ (impl_tac THEN1
-       (fs [Abbr‘tt’] \\ rename [‘SOME (find_var _ _,p1,l8)’]
-        \\ PairCases_on ‘l8’ \\ fs [call_env_def,push_env_def,isWord_def]
-        \\ pairarg_tac \\ fs [dec_clock_def,loopSemTheory.dec_clock_def,state_rel_def]))
-  \\ strip_tac \\ fs []
-  \\ Cases_on ‘res2’ \\ fs [] \\ rveq \\ fs []
-  \\ fs [loopSemTheory.dec_clock_def]
-  THEN1
+      >> pairarg_tac >> fs [pop_env_def,set_var_def]
+      >> imp_res_tac env_to_list_IMP
+      >> fs [loopSemTheory.set_var_def,loopSemTheory.dec_clock_def]
+      >> fs [state_rel_def]
+      >> rename [‘find_var ctxt var_name’]
+      >> ‘var_name IN domain ctxt’ by fs [assigned_vars_def]
+      >> simp [lookup_insert]
+      >> imp_res_tac find_var_neq_0 >> fs []
+      >> imp_res_tac cut_env_mk_new_cutset_IMP >> fs []
+      >> match_mp_tac locals_rel_insert >> fs []
+      >> fs [locals_rel_def])
+    >> qunabbrev_tac ‘tt’
+    >> pop_assum mp_tac
+    >> Cases_on ‘res1’ >- fs []
+    >> disch_then (fn th => assume_tac (REWRITE_RULE [IMP_DISJ_THM] th))
+    >> fs [] >> Cases_on ‘x’ >> fs []
+    >> fs [state_rel_def]
+    >> fs [call_env_def,push_env_def] >> pairarg_tac >> fs [dec_clock_def]
+    >> fs [jump_exc_def,NOT_LESS]
+    >> Cases_on ‘LENGTH t.stack <= t.handler’ >> fs [LASTN_ADD_CONS]
+    >> simp [CaseEq"option",CaseEq"prod",CaseEq"bool",set_var_def,CaseEq"list",
+             CaseEq"stack_frame"] >> rw [] >> fs [])
+  >> PairCases_on ‘x’ >> fs []
+  >> rpt (pairarg_tac >> fs [])
+  >> fs [evaluate_def,add_ret_loc_def,domain_mk_new_cutset_not_empty,cut_res_def]
+  >> fs [loopSemTheory.cut_state_def]
+  >> Cases_on ‘domain x1 ⊆ domain s.locals’ >> fs []
+  >> qpat_x_assum ‘locals_rel _ s.locals _’ assume_tac
+  >> drule cut_env_mk_new_cutset
+  >> rpt (disch_then drule) >> strip_tac >> fs []
+  >> (IF_CASES_TAC >> fs [] >- (rveq >> fs [flush_state_def,state_rel_def]))
+  >> fs [CaseEq"prod",CaseEq"option"] >> fs [] >> rveq >> fs []
+  >> rename [‘_ = (SOME res2,st)’]
+  >> qmatch_goalsub_abbrev_tac ‘wordSem$evaluate (_,tt)’
+  >> fs [PULL_EXISTS]
+  >> Cases_on ‘res2 = Error’ >> fs []
+  >> first_x_assum (qspecl_then [‘tt’,‘ctxt1’,‘Loc l0 l1’,‘l2’] mp_tac)
+  >> (impl_tac >-
+       (fs [Abbr‘tt’] >> rename [‘SOME (find_var _ _,p1,l8)’]
+        >> PairCases_on ‘l8’ >> fs [call_env_def,push_env_def,isWord_def]
+        >> pairarg_tac >> fs [dec_clock_def,loopSemTheory.dec_clock_def,state_rel_def]))
+  >> strip_tac >> fs []
+  >> Cases_on ‘res2’ >> fs [] >> rveq >> fs []
+  >> fs [loopSemTheory.dec_clock_def]
+  >-
    (rename [‘loopSem$set_var hvar w _’]
-    \\ Cases_on ‘evaluate (x2,set_var hvar w (st with locals := inter s.locals x1))’
-    \\ fs []
-    \\ Cases_on ‘q = SOME Error’ THEN1 fs [cut_res_def] \\ fs []
-    \\ fs [pop_env_def,Abbr‘tt’] \\ fs [call_env_def,push_env_def]
-    \\ rename [‘SOME (find_var _ _,p1,l8)’]
-    \\ PairCases_on ‘l8’ \\ fs [call_env_def,push_env_def]
-    \\ pairarg_tac \\ fs [dec_clock_def,loopSemTheory.dec_clock_def]
-    \\ pop_assum mp_tac
-    \\ pairarg_tac \\ fs [dec_clock_def,loopSemTheory.dec_clock_def]
-    \\ reverse IF_CASES_TAC THEN1 (imp_res_tac env_to_list_IMP \\ fs [])
-    \\ strip_tac \\ fs [] \\ pop_assum mp_tac \\ fs [set_var_def]
-    \\ fs [cut_res_def]
-    \\ qmatch_goalsub_abbrev_tac ‘wordSem$evaluate (_,tt)’ \\ strip_tac
-    \\ first_x_assum (qspecl_then [‘tt’,‘ctxt’,‘retv’,‘l1'’] mp_tac)
-    \\ impl_tac THEN1
+    >> Cases_on ‘evaluate (x2,set_var hvar w (st with locals := inter s.locals x1))’
+    >> fs []
+    >> Cases_on ‘q = SOME Error’ >- fs [cut_res_def] >> fs []
+    >> fs [pop_env_def,Abbr‘tt’] >> fs [call_env_def,push_env_def]
+    >> rename [‘SOME (find_var _ _,p1,l8)’]
+    >> PairCases_on ‘l8’ >> fs [call_env_def,push_env_def]
+    >> pairarg_tac >> fs [dec_clock_def,loopSemTheory.dec_clock_def]
+    >> pop_assum mp_tac
+    >> pairarg_tac >> fs [dec_clock_def,loopSemTheory.dec_clock_def]
+    >> reverse IF_CASES_TAC >- (imp_res_tac env_to_list_IMP >> fs [])
+    >> strip_tac >> fs [] >> pop_assum mp_tac >> fs [set_var_def]
+    >> fs [cut_res_def]
+    >> qmatch_goalsub_abbrev_tac ‘wordSem$evaluate (_,tt)’ >> strip_tac
+    >> first_x_assum (qspecl_then [‘tt’,‘ctxt’,‘retv’,‘l1'’] mp_tac)
+    >> impl_tac >-
      (fs [loopSemTheory.set_var_def,state_rel_def,Abbr‘tt’]
-      \\ qpat_x_assum ‘_ SUBSET domain ctxt’ mp_tac
-      \\ simp [assigned_vars_def]
-      \\ once_rewrite_tac [assigned_vars_acc]
-      \\ once_rewrite_tac [assigned_vars_acc] \\ fs [] \\ strip_tac
-      \\ qpat_x_assum ‘no_Loops (Call _ _ _ _)’ mp_tac
-      \\ simp [no_Loops_def,every_prog_def,no_Loop_def] \\ strip_tac
-      \\ imp_res_tac env_to_list_IMP \\ fs []
-      \\ fs [lookup_insert]
-      \\ imp_res_tac find_var_neq_0 \\ fs []
-      \\ imp_res_tac cut_env_mk_new_cutset_IMP \\ fs []
-      \\ match_mp_tac locals_rel_insert \\ fs [locals_rel_def])
-    \\ fs [] \\ strip_tac
-    \\ Cases_on ‘q’ \\ fs [] \\ rveq \\ fs []
-    THEN1
+      >> qpat_x_assum ‘_ SUBSET domain ctxt’ mp_tac
+      >> simp [assigned_vars_def]
+      >> once_rewrite_tac [assigned_vars_acc]
+      >> once_rewrite_tac [assigned_vars_acc] >> fs [] >> strip_tac
+      >> qpat_x_assum ‘no_Loops (Call _ _ _ _)’ mp_tac
+      >> simp [no_Loops_def,every_prog_def,no_Loop_def] >> strip_tac
+      >> imp_res_tac env_to_list_IMP >> fs []
+      >> fs [lookup_insert]
+      >> imp_res_tac find_var_neq_0 >> fs []
+      >> imp_res_tac cut_env_mk_new_cutset_IMP >> fs []
+      >> match_mp_tac locals_rel_insert >> fs [locals_rel_def])
+    >> fs [] >> strip_tac
+    >> Cases_on ‘q’ >> fs [] >> rveq >> fs []
+    >-
      (rename [‘cut_state names s9’]
-      \\ fs [loopSemTheory.cut_state_def]
-      \\ Cases_on ‘domain names ⊆ domain s9.locals’ \\ fs []
-      \\ imp_res_tac state_rel_IMP \\ fs []
-      \\ IF_CASES_TAC
-      \\ fs [flush_state_def] \\ rveq \\ fs [] \\ fs [state_rel_def,dec_clock_def]
-      \\ fs [loopSemTheory.dec_clock_def,Abbr‘tt’]
-      \\ fs [locals_rel_def,lookup_inter_alt])
-    \\ Cases_on ‘x’ \\ fs []
-    THEN1 fs [Abbr‘tt’]
-    \\ pop_assum mp_tac \\ rewrite_tac [IMP_DISJ_THM]
-    \\ IF_CASES_TAC \\ fs []
-    \\ fs [Abbr‘tt’] \\ metis_tac [])
-  THEN1
+      >> fs [loopSemTheory.cut_state_def]
+      >> Cases_on ‘domain names ⊆ domain s9.locals’ >> fs []
+      >> imp_res_tac state_rel_IMP >> fs []
+      >> IF_CASES_TAC
+      >> fs [flush_state_def] >> rveq >> fs [] >> fs [state_rel_def,dec_clock_def]
+      >> fs [loopSemTheory.dec_clock_def,Abbr‘tt’]
+      >> fs [locals_rel_def,lookup_inter_alt])
+    >> Cases_on ‘x’ >> fs []
+    >- fs [Abbr‘tt’]
+    >> pop_assum mp_tac >> rewrite_tac [IMP_DISJ_THM]
+    >> IF_CASES_TAC >> fs []
+    >> fs [Abbr‘tt’] >> metis_tac [])
+  >-
    (qpat_x_assum ‘∀x. _’ (assume_tac o REWRITE_RULE [IMP_DISJ_THM])
-    \\ rename [‘loopSem$set_var hvar w _’]
-    \\ Cases_on ‘evaluate (x1',set_var hvar w (st with locals := inter s.locals x1))’
-    \\ fs []
-    \\ Cases_on ‘q = SOME Error’ THEN1 fs [cut_res_def] \\ fs []
-    \\ fs [pop_env_def,Abbr‘tt’] \\ fs [call_env_def,push_env_def]
-    \\ rename [‘SOME (find_var _ _,p1,l8)’]
-    \\ PairCases_on ‘l8’ \\ fs [call_env_def,push_env_def]
-    \\ pairarg_tac \\ fs [dec_clock_def,loopSemTheory.dec_clock_def]
-    \\ pop_assum mp_tac
-    \\ pairarg_tac \\ fs [dec_clock_def,loopSemTheory.dec_clock_def]
-    \\ Cases_on ‘res1’ \\ fs [] \\ rveq \\ fs []
-    \\ qpat_x_assum ‘∀x. _’ mp_tac
-    \\ simp [jump_exc_def]
-    \\ qmatch_goalsub_abbrev_tac ‘LASTN n1 xs1’
-    \\ ‘LASTN n1 xs1 = xs1’  by
-       (qsuff_tac ‘n1 = LENGTH xs1’ \\ fs [LASTN_LENGTH_ID]
-        \\ unabbrev_all_tac \\ fs [])
-    \\ fs [] \\ fs [Abbr‘n1’,Abbr‘xs1’] \\ strip_tac \\ rveq \\ fs []
-    \\ ‘t1.locals = fromAList l ∧
+    >> rename [‘loopSem$set_var hvar w _’]
+    >> Cases_on ‘evaluate (x1',set_var hvar w (st with locals := inter s.locals x1))’
+    >> fs []
+    >> Cases_on ‘q = SOME Error’ >- fs [cut_res_def] >> fs []
+    >> fs [pop_env_def,Abbr‘tt’] >> fs [call_env_def,push_env_def]
+    >> rename [‘SOME (find_var _ _,p1,l8)’]
+    >> PairCases_on ‘l8’ >> fs [call_env_def,push_env_def]
+    >> pairarg_tac >> fs [dec_clock_def,loopSemTheory.dec_clock_def]
+    >> pop_assum mp_tac
+    >> pairarg_tac >> fs [dec_clock_def,loopSemTheory.dec_clock_def]
+    >> Cases_on ‘res1’ >> fs [] >> rveq >> fs []
+    >> qpat_x_assum ‘∀x. _’ mp_tac
+    >> simp [jump_exc_def]
+    >> qmatch_goalsub_abbrev_tac ‘LASTN n1 xs1’
+    >> ‘LASTN n1 xs1 = xs1’  by
+       (qsuff_tac ‘n1 = LENGTH xs1’ >> fs [LASTN_LENGTH_ID]
+        >> unabbrev_all_tac >> fs [])
+    >> fs [] >> fs [Abbr‘n1’,Abbr‘xs1’] >> strip_tac >> rveq >> fs []
+    >> ‘t1.locals = fromAList l ∧
         t1.stack = t.stack ∧ t1.handler = t.handler’ by fs [state_component_equality]
-    \\ reverse IF_CASES_TAC THEN1 (imp_res_tac env_to_list_IMP \\ fs [] \\ rfs [])
-    \\ strip_tac \\ fs []
-    \\ pop_assum mp_tac \\ fs [set_var_def]
-    \\ fs [cut_res_def]
-    \\ qmatch_goalsub_abbrev_tac ‘wordSem$evaluate (_,tt)’ \\ strip_tac
-    \\ first_x_assum (qspecl_then [‘tt’,‘ctxt’,‘retv’,‘(l0,l1 + 1)’] mp_tac)
-    \\ impl_tac THEN1
+    >> reverse IF_CASES_TAC >- (imp_res_tac env_to_list_IMP >> fs [] >> rfs [])
+    >> strip_tac >> fs []
+    >> pop_assum mp_tac >> fs [set_var_def]
+    >> fs [cut_res_def]
+    >> qmatch_goalsub_abbrev_tac ‘wordSem$evaluate (_,tt)’ >> strip_tac
+    >> first_x_assum (qspecl_then [‘tt’,‘ctxt’,‘retv’,‘(l0,l1 + 1)’] mp_tac)
+    >> impl_tac >-
      (fs [loopSemTheory.set_var_def,state_rel_def,Abbr‘tt’]
-      \\ qpat_x_assum ‘_ SUBSET domain ctxt’ mp_tac
-      \\ simp [assigned_vars_def]
-      \\ once_rewrite_tac [assigned_vars_acc]
-      \\ once_rewrite_tac [assigned_vars_acc] \\ fs [] \\ strip_tac
-      \\ qpat_x_assum ‘no_Loops (Call _ _ _ _)’ mp_tac
-      \\ simp [no_Loops_def,every_prog_def,no_Loop_def] \\ strip_tac
-      \\ imp_res_tac env_to_list_IMP \\ fs []
-      \\ fs [lookup_insert]
-      \\ imp_res_tac find_var_neq_0 \\ fs []
-      \\ imp_res_tac cut_env_mk_new_cutset_IMP \\ fs []
-      \\ match_mp_tac locals_rel_insert \\ fs [locals_rel_def])
-    \\ fs [] \\ strip_tac
-    \\ Cases_on ‘q’ \\ fs [] \\ rveq \\ fs []
-    THEN1
+      >> qpat_x_assum ‘_ SUBSET domain ctxt’ mp_tac
+      >> simp [assigned_vars_def]
+      >> once_rewrite_tac [assigned_vars_acc]
+      >> once_rewrite_tac [assigned_vars_acc] >> fs [] >> strip_tac
+      >> qpat_x_assum ‘no_Loops (Call _ _ _ _)’ mp_tac
+      >> simp [no_Loops_def,every_prog_def,no_Loop_def] >> strip_tac
+      >> imp_res_tac env_to_list_IMP >> fs []
+      >> fs [lookup_insert]
+      >> imp_res_tac find_var_neq_0 >> fs []
+      >> imp_res_tac cut_env_mk_new_cutset_IMP >> fs []
+      >> match_mp_tac locals_rel_insert >> fs [locals_rel_def])
+    >> fs [] >> strip_tac
+    >> Cases_on ‘q’ >> fs [] >> rveq >> fs []
+    >-
      (rename [‘cut_state names s9’]
-      \\ fs [loopSemTheory.cut_state_def]
-      \\ Cases_on ‘domain names ⊆ domain s9.locals’ \\ fs []
-      \\ imp_res_tac state_rel_IMP \\ fs []
-      \\ IF_CASES_TAC
-      \\ fs [flush_state_def] \\ rveq \\ fs [] \\ fs [state_rel_def,dec_clock_def]
-      \\ fs [loopSemTheory.dec_clock_def,Abbr‘tt’]
-      \\ fs [locals_rel_def,lookup_inter_alt])
-    \\ pop_assum (assume_tac o REWRITE_RULE [IMP_DISJ_THM])
-    \\ Cases_on ‘x’ \\ fs []
-    THEN1 fs [Abbr‘tt’]
-    \\ rveq \\ fs []
-    \\ pop_assum mp_tac
-    \\ fs [Abbr‘tt’,jump_exc_def]
-    \\ metis_tac [])
+      >> fs [loopSemTheory.cut_state_def]
+      >> Cases_on ‘domain names ⊆ domain s9.locals’ >> fs []
+      >> imp_res_tac state_rel_IMP >> fs []
+      >> IF_CASES_TAC
+      >> fs [flush_state_def] >> rveq >> fs [] >> fs [state_rel_def,dec_clock_def]
+      >> fs [loopSemTheory.dec_clock_def,Abbr‘tt’]
+      >> fs [locals_rel_def,lookup_inter_alt])
+    >> pop_assum (assume_tac o REWRITE_RULE [IMP_DISJ_THM])
+    >> Cases_on ‘x’ >> fs []
+    >- fs [Abbr‘tt’]
+    >> rveq >> fs []
+    >> pop_assum mp_tac
+    >> fs [Abbr‘tt’,jump_exc_def]
+    >> metis_tac [])
 QED
 
 Theorem compile_correct:
   ^(compile_correct_tm())
 Proof
   match_mp_tac (the_ind_thm())
-  \\ EVERY (map strip_assume_tac [compile_Skip, compile_Raise,
+  >> EVERY (map strip_assume_tac [compile_Skip, compile_Raise,
        compile_Mark, compile_Return, compile_Assign, compile_Store,
        compile_SetGlobal, compile_Call, compile_Seq, compile_If,
        compile_FFI, compile_Loop, compile_LoadByte])
-  \\ asm_rewrite_tac [] \\ rw [] \\ rpt (pop_assum kall_tac)
+  >> asm_rewrite_tac [] >> rw [] >> rpt (pop_assum kall_tac)
 QED
 
 val _ = export_theory();
